% !TeX root = ./TMA03.tex
\begin{question}
Given that $a, b, c$ are constant with $a > 0$, $b > 0$, $c > 0$, it will be shown that the stationary path of the functional
\[
	S[y] = \Int{0}{a}{x} \lr{y^{\prime 2} + 2b y},\quad y(a) = 0,
\]
with a natural boundary condition at $x = 0$ and subject to the constraint
\[
	C[y] = \Int{0}{a}{x} y = c,
\]
is given by
\[
	y(x) = \frac{3c}{2a^3}\lr{a^2-x^2},
\]
as follows.
The \el is given by
\[
	\EL.
\]
Now, 
\[
	\overline{F} = y^{\prime 2} + 2b y -\lambda y,\quad\text{where } \lambda\text{ is a Lagrange multiplier.}
\]
\[
	\overline{F}_y = \pderiv{\overline{F}}{y} =2b -\lambda\quad\text{ and } \overline{F}_{y^\prime} = \pderiv{\overline{F}}{y^\prime} = 2y^\prime.
\]
The \el becomes
\begin{align*}
 	\deriv{}{x}\lr{2y^\prime}-\lr{2b-\lambda} = 0,\\
 	2y^{\prime\prime} - 2b + \lambda = 0.
\end{align*}
Hence,
\begin{align*}
	y^{\prime\prime}=& b-\dfrac{\lambda}{2},\\
	y^{\prime}=& \lr{b-\dfrac{\lambda}{2}}x+c_1 \text{ and}\\
	y=& \lr{\dfrac{b-\lambda/2}{2}}x^2 + c_1x + c_2, \text{ where  $c_1$ and $c_2$ are arbitrary constants}. 
\end{align*}  
Applying the boundary condition $y(a)=0$
 \[
 	y(a)=\lr{\dfrac{b-\lambda/2}{2}}a^2 + c_1a + c_2=0.
 \]
 The \el must also satisfy the extra boundary condition $\overline{F}_{y^\prime}=0$ at $x=0$, thus
 \begin{align*}
 	\overline{F}_{y^\prime} =& 2y^\prime = 0\quad\text{and}\quad y^\prime(0) = 0.\\
 	y^\prime(x) =& \lr{b-\frac{\lambda}{2}}x + c_1,\\
 	y^\prime(0) =& \lr{b-\frac{\lambda}{2}}(0) + c_1=0,\quad\text{thus,}\quad c_1=0.\\
 \end{align*}
Hence,
\begin{align*}
 	y=& \lr{\dfrac{b-\lambda/2}{2}}x^2 + c_2, \quad\text{where}\quad c_2 =-\lr{\dfrac{b-\lambda/2}{2}}a^2.\\
 	\text{So, } y=& \lr{\dfrac{b-\lambda/2}{2}}\lr{x^2-a^2}.
\end{align*}
Now, given the constraint
\begin{align*}
	C\lrs{y} = \Int{0}{a}{x} y =& c,\\
\Int{0}{a}{x}\lr{\dfrac{b-\lambda/2}{2}}\lr{x^2-a^2} =& c,\\
\lr{\dfrac{b-\lambda/2}{2}} \Int{0}{a}{x}\lr{x^2-a^2} =& c,\\
\lr{\dfrac{b-\lambda/2}{2}}\lrs{\frac{x^3}{3}-a^2x}_0^a=&c,\\
\lr{\dfrac{b-\lambda/2}{2}}\lr{\frac{a^3}{3}-a^3} =& c,\\
\lr{\dfrac{b-\lambda/2}{2}}\lr{\frac{-2a^3}{3}} =& c,\\
\lr{b-\frac{\lambda}{2}}\lr{\frac{-a^3}{3}} =& c,\\
-\lr{b-\frac{\lambda}{2}}\lr{\frac{a^3}{3}} =& c.
\end{align*}
Thus, 
\[b-\dfrac{\lambda}{2} = -\dfrac{3c}{a^3}\] and \[y=-\dfrac{3c}{2a^3}\lr{x^2-a^2}.\]
Thus, \[y=\dfrac{3c}{2a^3}\lr{a^2-x^2}, \text{ as required}.\]
\end{question}
